---
title: 类欧几里得算法学习笔记
date: 2018-10-18 13:14:58
tags: [类欧几里得算法, 学习笔记]
categories: 学习笔记（OI/XCPC）
---

常见的用类欧几里得算法处理的几个函数：

$$
f(a, b, c, n) = \sum_{i = 0}^{n} \lfloor \frac{ai + b}{c} \rfloor
$$
$$
g(a, b, c, n) = \sum_{i = 0}^{n} i\lfloor \frac{ai + b}{c} \rfloor
$$
$$
h(a, b, c, n) = \sum_{i = 0}^{n} \lfloor \frac{ai + b}{c} \rfloor ^2
$$

并定义：

$$
m = \lfloor \frac{an + b}{c} \rfloor
$$

可在 $O(\log \min(a, b))$ 的时间内计算以上函数。

<!-- more -->

## 函数 $f$ 的处理

当 $a \geq c$ 或 $b \geq c$ 时：

$$
\begin{align}
f(a, b, c, n) &= \sum_{i = 0}^{n} \left( \lfloor \frac{i (a \bmod c) + b \bmod c}{c} \rfloor + \lfloor \frac{a}{c} \rfloor i + \lfloor \frac{b}{c} \rfloor \right) \\
&= f(a \bmod c, b \bmod c, c, n) + \lfloor \frac{a}{c} \rfloor \frac{n(n + 1)}{2} + (n + 1) \lfloor \frac{b}{c} \rfloor
\end{align}
$$

当 $a < c$ 且 $b < c$ 时：

$$
\begin{align}
f(a, b, c, n) &= \sum_{i = 0}^{n} \sum_{j = 1}^{m} [\frac{ai + b}{c} \geq j] \\
&= \sum_{i = 0}^{n} \sum_{j = 0}^{m - 1} [ai \geq c(j + 1) - b] \\
&= \sum_{i = 0}^{n} \sum_{j = 0}^{m - 1} [ai > cj + c - b - 1] \\
&= \sum_{i = 0}^{n} \sum_{j = 0}^{m - 1} [i > \frac{cj + c - b - 1}{a}] \\
&= \sum_{j = 0}^{m - 1} \sum_{i = 0}^{n} [i > \frac{cj + c - b - 1}{a}] \\
&= \sum_{j = 0}^{m - 1} \left( n - \lfloor \frac{cj + c - b - 1}{a} \rfloor \right) \\
&= nm - f(c, c - b - 1, a, m - 1)
\end{align}
$$

## 函数 $g$ 的处理

当 $a \geq c$ 或 $b \geq c$ 时：

$$
\begin{align}
g(a, b, c, n) &= \sum_{i = 0}^{n} \left( \lfloor \frac{i (a \bmod c) + b \bmod c}{c} \rfloor i + \lfloor \frac{a}{c} \rfloor i^2 + \lfloor \frac{b}{c} \rfloor i \right) \\
&= g(a \bmod c, b \bmod c, c, n) + \lfloor \frac{a}{c} \rfloor \frac{n(n + 1)(2n + 1)}{6} + \lfloor \frac{b}{c} \rfloor \frac{n(n + 1)}{2}
\end{align}
$$

当 $a < c$ 且 $b < c$ 时：

$$
\begin{align}
g(a, b, c, n) &= \sum_{i = 0}^{n} i \sum_{j = 1}^{m} [\frac{ai + b}{c} \geq j] \\
&= \sum_{i = 0}^{n} i \sum_{j = 0}^{m - 1} [i > \frac{cj + c - b - 1}{a}] \\
&= \sum_{j = 0}^{m - 1} \sum_{i = 0}^{n} i [i > \frac{cj + c - b - 1}{a}] \\
&= \sum_{j = 0}^{m - 1} \frac{1}{2} (n + 1 + \lfloor \frac{cj + c - b - 1}{a} \rfloor) (n - \lfloor \frac{cj + c - b - 1}{a} \rfloor) \\
&= \frac{1}{2} \sum_{j = 0}^{m - 1} \left(n(n + 1) - \lfloor \frac{cj + c - b - 1}{a} \rfloor - \lfloor \frac{cj + c - b - 1}{a} \rfloor ^2 \right) \\
&= \frac{1}{2} \left( nm(n + 1) - f(c, c - b - 1, a, m - 1) - h(c, c - b - 1, a, m - 1) \right)
\end{align}
$$

## 函数 $h$ 的处理

当 $a \geq c$ 或 $b \geq c$ 时：

$$
\begin{align}
h(a, b, c, n) &= \sum_{i = 0}^{n} \left( \lfloor \frac{i (a \bmod c) + b \bmod c}{c} \rfloor + \lfloor \frac{a}{c} \rfloor i + \lfloor \frac{b}{c} \rfloor \right)^2 \\
&= h(a \bmod c, b \bmod c, c, n) + 2 \lfloor \frac{a}{c} \rfloor g(a \bmod c, b \bmod c, c, n) + 2 \lfloor \frac{b}{c} \rfloor f(a \bmod c, b  \bmod c, c, n) \\
&+ \lfloor \frac{a}{c} \rfloor^2 \frac{n(n + 1)(2n + 1)}{6} + \lfloor \frac{b}{c} \rfloor^2(n + 1) + \lfloor \frac{a}{c} \rfloor \lfloor \frac{b}{c} \rfloor n(n + 1)
\end{align}
$$

当 $a < c$ 且 $b < c$ 时：

$$
\begin{align}
\because ~&
n^2 = 2 \times \frac{n(n + 1)}{2} - n = 2\sum_{i = 1}^{n}i - n \\
\therefore ~&
h(a, b, c, n) = \sum_{i = 0}^{n} (2 \sum_{j = 1}^{\lfloor \frac{ai + b}{c} \rfloor} j - \lfloor \frac{ai + b}{c} \rfloor)
\end{align}
$$
$$
\begin{align}
h(a, b, c, n) &= \sum_{i = 0}^{n} (2 \sum_{j = 1}^{\lfloor \frac{ai + b}{c} \rfloor} j - \lfloor \frac{ai + b}{c} \rfloor) \\
&= 2 \sum_{j = 0}^{m - 1} (j + 1) \sum_{i = 0}^{n} [\frac{ai + b}{c} \geq j + 1] - f(a, b, c, n) \\
&= 2 \sum_{j = 0}^{m - 1} (j + 1) \sum_{i = 0}^{n} [i > \frac{cj + c - b - 1}{a}] - f(a, b, c, n) \\
&= 2 \sum_{j = 0}^{m - 1} (j + 1) (n - \lfloor \frac{cj + c - b - 1}{a} \rfloor) - f(a, b, c, n) \\
&= nm(m + 1) - 2g(c, c - b - 1, a, m - 1) - f(a, b, c, n)
\end{align}
$$

